LeanWang.lean
@@ -4,4 +4,5 @@ import LeanWang.FiniteSearchProgram
 import LeanWang.FuelMachine
 import LeanWang.Machine
 import LeanWang.MachineTiles
+import LeanWang.ToPartrecEncoding
 import LeanWang.Theorems
